add memory to asm

theories/asm.v
@@ -8,42 +8,62 @@ Require Import refframe.proof_techniques.
 Local Open Scope Z_scope.
 (** * Assembly language *)
 Inductive asm_instr_event :=
-| WriteReg (r : string) (f : gmap string Z → Z).
+| WriteReg (r : string) (f : gmap string Z → Z)
+(* ldr r1, [f r2] *)
+| ReadMem (r1 r2 : string) (f : Z → Z)
+(* str r1, [f r2] *)
+| WriteMem (r1 r2 : string) (f : Z → Z)
+.
 
 Definition asm_instr := list asm_instr_event.
 
 Inductive asm_state := AsmState {
   asm_cur_instr : option asm_instr;
   asm_regs : gmap string Z;
+  asm_mem : gmap Z Z;
   asm_instrs : gmap Z asm_instr;
 }.
 Add Printing Constructor asm_state.
 
-Definition initial_asm_state (instrs : gmap Z asm_instr) := AsmState None ∅ instrs.
+Definition initial_asm_state (instrs : gmap Z asm_instr) := AsmState None ∅ ∅ instrs.
 
 Inductive asm_event :=
-| EAJump (pc : Z) (regs : gmap string Z)
-| EARecvJump (pc : Z) (regs : gmap string Z).
+| EAJump (pc : Z) (regs : gmap string Z) (mem : gmap Z Z)
+| EARecvJump (pc : Z) (regs : gmap string Z) (mem : gmap Z Z).
 
 Inductive asm_step : asm_state → option asm_event → (asm_state → Prop) → Prop :=
-| SWriteReg regs instrs r f es:
-  asm_step (AsmState (Some (WriteReg r f :: es)) regs instrs) None
-           (λ σ', is_Some (regs !! r) ∧ σ' = AsmState (Some es) (<[r := f regs]>regs) instrs)
-| SJumpInternal regs instrs pc es :
+| SWriteReg regs instrs r f es mem:
+  asm_step (AsmState (Some (WriteReg r f :: es)) regs mem instrs) None (λ σ',
+         is_Some (regs !! r) ∧
+         σ' = AsmState (Some es) (<[r := f regs]>regs) mem instrs)
+| SReadMem regs instrs r1 r2 f es mem:
+  asm_step (AsmState (Some (ReadMem r1 r2 f :: es)) regs mem instrs) None (λ σ', ∃ a,
+         regs !! r2 = Some a ∧
+         (* mem !! f a = Some v ∧ *)
+         is_Some (regs !! r1) ∧
+         σ' = AsmState (Some es) (<[r1 := mem !!! f a]>regs) mem instrs)
+| SWriteMem regs instrs r1 r2 f es mem:
+  asm_step (AsmState (Some (WriteMem r1 r2 f :: es)) regs mem instrs) None (λ σ', ∃ a v,
+         regs !! r2 = Some a ∧
+         regs !! r1 = Some v ∧
+         (* TODO: Should we have the following constraint? *)
+         (* is_Some (mem !! f a) ∧ *)
+         σ' = AsmState (Some es) regs (<[f a := v]>mem) instrs)
+| SJumpInternal regs instrs pc es mem:
   regs !! "PC" = Some pc →
   instrs !! pc = Some es →
-  asm_step (AsmState (Some []) regs instrs) None
-           (λ σ', σ' = AsmState (Some es) regs instrs)
-| SJumpExternal regs instrs pc :
+  asm_step (AsmState (Some []) regs mem instrs) None
+           (λ σ', σ' = AsmState (Some es) regs mem instrs)
+| SJumpExternal regs instrs pc mem:
   regs !! "PC" = Some pc →
   instrs !! pc = None →
-  asm_step (AsmState (Some []) regs instrs) (Some (EAJump pc regs))
-           (λ σ', σ' = AsmState None regs instrs)
-| SRecvJump regs regs' instrs pc es :
+  asm_step (AsmState (Some []) regs mem instrs) (Some (EAJump pc regs mem))
+           (λ σ', σ' = AsmState None regs mem instrs)
+| SRecvJump regs regs' instrs pc es mem mem':
   regs' !! "PC" = Some pc →
   instrs !! pc = Some es →
-  asm_step (AsmState None regs instrs) (Some (EARecvJump pc regs'))
-           (λ σ', σ' = AsmState (Some es) regs' instrs)
+  asm_step (AsmState None regs mem instrs) (Some (EARecvJump pc regs' mem'))
+           (λ σ', σ' = AsmState (Some es) regs' mem' instrs)
 .
 
 Definition asm_module := Mod asm_step.
@@ -55,9 +75,9 @@ Proof. move => *. invert_all @m_step; naive_solver. Qed.
 (** * tstep *)
 Global Hint Transparent asm_instr : tstep.
 
-Lemma asm_step_WriteReg_i r f es rs ins:
-  TStepI asm_module (AsmState (Some (WriteReg r f::es)) rs ins)
-            (λ G, G true None (λ G', is_Some (rs !! r) ∧ G' (AsmState (Some (es)) (<[r:=f rs]>rs) ins))).
+Lemma asm_step_WriteReg_i r f es rs ins mem:
+  TStepI asm_module (AsmState (Some (WriteReg r f::es)) rs mem ins)
+            (λ G, G true None (λ G', is_Some (rs !! r) ∧ G' (AsmState (Some (es)) (<[r:=f rs]>rs) mem ins))).
 Proof.
   constructor => ? ?. apply steps_impl_step_end => ???.
   invert_all @m_step. eexists _, _. split_and!; [done|done|].
@@ -65,9 +85,9 @@ Proof.
 Qed.
 Global Hint Resolve asm_step_WriteReg_i : tstep.
 
-Lemma asm_step_WriteReg_s r f es rs ins:
-  TStepS asm_module (AsmState (Some (WriteReg r f::es)) rs ins)
-            (λ G, G None (λ G', is_Some (rs !! r) → G' (AsmState (Some (es)) (<[r:=f rs]>rs) ins))).
+Lemma asm_step_WriteReg_s r f es rs ins mem:
+  TStepS asm_module (AsmState (Some (WriteReg r f::es)) rs mem ins)
+            (λ G, G None (λ G', is_Some (rs !! r) → G' (AsmState (Some (es)) (<[r:=f rs]>rs) mem ins))).
 Proof.
   constructor => ??. eexists _, _. split; [done|] => ? /= ?.
   apply: steps_spec_step_end. { econs. }
@@ -75,13 +95,55 @@ Proof.
 Qed.
 Global Hint Resolve asm_step_WriteReg_s : tstep.
 
-Lemma asm_step_Jump_i rs ins:
-  TStepI asm_module (AsmState (Some []) rs ins) (λ G,
+Lemma asm_step_ReadMem_i r1 r2 f es rs ins mem:
+  TStepI asm_module (AsmState (Some (ReadMem r1 r2 f::es)) rs mem ins)
+            (λ G, G true None (λ G',
+             ∃ a, rs !! r2 = Some a ∧ is_Some (rs !! r1) ∧ G' (AsmState (Some es) (<[r1:=mem !!! f a]>rs) mem ins))).
+Proof.
+  constructor => ? ?. apply steps_impl_step_end => ???.
+  invert_all @m_step. eexists _, _. split_and!; [done|done|].
+  move => ? /=. naive_solver.
+Qed.
+Global Hint Resolve asm_step_ReadMem_i : tstep.
+
+Lemma asm_step_ReadMem_s r1 r2 f es rs ins mem:
+  TStepS asm_module (AsmState (Some (ReadMem r1 r2 f::es)) rs mem ins)
+            (λ G, G None (λ G', ∀ a, rs !! r2 = Some a → is_Some (rs !! r1) → G' (AsmState (Some (es)) (<[r1:=mem !!! f a]>rs) mem ins))).
+Proof.
+  constructor => ??. eexists _, _. split; [done|] => ? /= ?.
+  apply: steps_spec_step_end. { econs. }
+  move => ? /= [? [? [? ->]]]. naive_solver.
+Qed.
+Global Hint Resolve asm_step_ReadMem_s : tstep.
+
+Lemma asm_step_WriteMem_i r1 r2 f es rs ins mem:
+  TStepI asm_module (AsmState (Some (WriteMem r1 r2 f::es)) rs mem ins)
+            (λ G, G true None (λ G',
+             ∃ a v, rs !! r2 = Some a ∧ rs !! r1 = Some v ∧ G' (AsmState (Some es) rs (<[f a:=v]>mem) ins))).
+Proof.
+  constructor => ? ?. apply steps_impl_step_end => ???.
+  invert_all @m_step. eexists _, _. split_and!; [done|done|].
+  move => ? /=. naive_solver.
+Qed.
+Global Hint Resolve asm_step_WriteMem_i : tstep.
+
+Lemma asm_step_WriteMem_s r1 r2 f es rs ins mem:
+  TStepS asm_module (AsmState (Some (WriteMem r1 r2 f::es)) rs mem ins)
+            (λ G, G None (λ G', ∀ a v, rs !! r2 = Some a → rs !! r1 = Some v → G' (AsmState (Some es) rs (<[f a:=v]>mem) ins))).
+Proof.
+  constructor => ??. eexists _, _. split; [done|] => ? /= ?.
+  apply: steps_spec_step_end. { econs. }
+  move => ? /= [? [? [? [? ->]]]]. naive_solver.
+Qed.
+Global Hint Resolve asm_step_WriteMem_s : tstep.
+
+Lemma asm_step_Jump_i rs ins mem:
+  TStepI asm_module (AsmState (Some []) rs mem ins) (λ G,
     ∀ pc, rs !! "PC" = Some pc →
           if ins !! pc is Some i then
-            G true None (λ G', G' (AsmState (Some i) (rs) ins))
+            G true None (λ G', G' (AsmState (Some i) rs mem ins))
           else
-            G true (Some (EAJump pc rs)) (λ G', G' (AsmState None (rs) ins))
+            G true (Some (EAJump pc rs mem)) (λ G', G' (AsmState None rs mem ins))
    ).
 Proof.
   constructor => ? HG. apply steps_impl_step_end => ???.
@@ -90,13 +152,13 @@ Proof.
 Qed.
 Global Hint Resolve asm_step_Jump_i : tstep.
 
-Lemma asm_step_Jump_s rs ins:
-  TStepS asm_module (AsmState (Some []) rs ins) (λ G,
+Lemma asm_step_Jump_s rs ins mem:
+  TStepS asm_module (AsmState (Some []) rs mem ins) (λ G,
     ∃ pc, rs !! "PC" = Some pc ∧
       if ins !! pc is Some i then
-        G None (λ G', G' (AsmState (Some i) (rs) ins))
+        G None (λ G', G' (AsmState (Some i) rs mem ins))
       else
-        G (Some (EAJump pc rs)) (λ G', G' (AsmState None rs ins))).
+        G (Some (EAJump pc rs mem)) (λ G', G' (AsmState None rs mem ins))).
 Proof.
   constructor => ?[?[??]]. case_match.
   all: eexists _, _; split; [done|] => ? /= ?.
@@ -104,11 +166,12 @@ Proof.
 Qed.
 Global Hint Resolve asm_step_Jump_s : tstep.
 
-Lemma asm_step_None_i rs ins:
-  TStepI asm_module (AsmState None rs ins) (λ G,
-    ∀ pc i rs', rs' !! "PC" = Some pc →
+Lemma asm_step_None_i rs ins mem:
+  TStepI asm_module (AsmState None rs mem ins) (λ G,
+    ∀ pc i rs' mem',
+      rs' !! "PC" = Some pc →
       ins !! pc = Some i →
-      G true (Some (EARecvJump pc rs')) (λ G', G' (AsmState (Some i) rs' ins))
+      G true (Some (EARecvJump pc rs' mem')) (λ G', G' (AsmState (Some i) rs' mem' ins))
    ).
 Proof.
   constructor => ? HG. apply steps_impl_step_end => ???.
@@ -116,11 +179,11 @@ Proof.
 Qed.
 Global Hint Resolve asm_step_None_i : tstep.
 
-Lemma asm_step_None_s rs ins:
-  TStepS asm_module (AsmState None rs ins) (λ G,
-    ∃ pc i rs', rs' !! "PC" = Some pc ∧
+Lemma asm_step_None_s rs mem ins:
+  TStepS asm_module (AsmState None rs mem ins) (λ G,
+    ∃ pc i rs' mem', rs' !! "PC" = Some pc ∧
       ins !! pc = Some i ∧
-      G (Some (EARecvJump pc rs')) (λ G', G' (AsmState (Some i) rs' ins))).
+      G (Some (EARecvJump pc rs' mem')) (λ G', G' (AsmState (Some i) rs' mem' ins))).
 Proof.
   constructor => ??. destruct_all!. eexists _, _. split; [done|] => ? /= ?.
   apply: steps_spec_step_end. { by econs. } naive_solver.
@@ -138,40 +201,41 @@ Definition asm_ctx_refines (instrsi instrss : gmap Z asm_instr) :=
 (** * semantic linking *)
 Inductive asm_prod_filter_state :=
 | APFLeft | APFRight | APFNone
-| APFRecvL (pc : Z) (rs : gmap string Z) | APFRecvR (pc : Z) (rs : gmap string Z).
+| APFRecvL (pc : Z) (rs : gmap string Z) (mem : gmap Z Z)
+ | APFRecvR (pc : Z) (rs : gmap string Z) (mem : gmap Z Z).
 
 Inductive asm_prod_filter (ins1 ins2 : gset Z) :
   asm_prod_filter_state → (seq_product_event asm_event asm_event) → option asm_event → asm_prod_filter_state →  Prop :=
-| APFJumpRecvL pc rs:
+| APFJumpRecvL pc rs mem:
   pc ∉ ins1 →
   pc ∈ ins2 →
-  asm_prod_filter ins1 ins2 APFLeft (SPELeft (EAJump pc rs) SPRight) None (APFRecvR pc rs)
-| APFJumpRecvL2 pc rs:
-  asm_prod_filter ins1 ins2 (APFRecvR pc rs) (SPERight (EARecvJump pc rs) SPRight) None APFRight
-| APFJumpRecvR pc rs:
+  asm_prod_filter ins1 ins2 APFLeft (SPELeft (EAJump pc rs mem) SPRight) None (APFRecvR pc rs mem)
+| APFJumpRecvL2 pc rs mem:
+  asm_prod_filter ins1 ins2 (APFRecvR pc rs mem) (SPERight (EARecvJump pc rs mem) SPRight) None APFRight
+| APFJumpRecvR pc rs mem:
   pc ∈ ins1 →
   pc ∉ ins2 →
-  asm_prod_filter ins1 ins2 APFRight (SPERight (EAJump pc rs) SPLeft) None (APFRecvL pc rs)
-| APFJumpRecvR2 pc rs:
-  asm_prod_filter ins1 ins2 (APFRecvL pc rs) (SPELeft (EARecvJump pc rs) SPLeft) None APFLeft
-| APFJumpExtL pc rs:
+  asm_prod_filter ins1 ins2 APFRight (SPERight (EAJump pc rs mem) SPLeft) None (APFRecvL pc rs mem)
+| APFJumpRecvR2 pc rs mem:
+  asm_prod_filter ins1 ins2 (APFRecvL pc rs mem) (SPELeft (EARecvJump pc rs mem) SPLeft) None APFLeft
+| APFJumpExtL pc rs mem:
   pc ∉ ins1 →
   pc ∉ ins2 →
-  asm_prod_filter ins1 ins2 APFLeft (SPELeft (EAJump pc rs) SPNone) (Some (EAJump pc rs)) APFNone
-| APFJumpExtR pc rs:
+  asm_prod_filter ins1 ins2 APFLeft (SPELeft (EAJump pc rs mem) SPNone) (Some (EAJump pc rs mem)) APFNone
+| APFJumpExtR pc rs mem:
   pc ∉ ins1 →
   pc ∉ ins2 →
-  asm_prod_filter ins1 ins2 APFRight (SPERight (EAJump pc rs) SPNone) (Some (EAJump pc rs)) APFNone
-| APFRecvJumpL pc rs:
+  asm_prod_filter ins1 ins2 APFRight (SPERight (EAJump pc rs mem) SPNone) (Some (EAJump pc rs mem)) APFNone
+| APFRecvJumpL pc rs mem:
   pc ∈ ins1 →
   pc ∉ ins2 →
   rs !! "PC" = Some pc →
-  asm_prod_filter ins1 ins2 APFNone (SPENone SPLeft) (Some (EARecvJump pc rs)) (APFRecvL pc rs)
-| APFRecvJumpR pc rs:
+  asm_prod_filter ins1 ins2 APFNone (SPENone SPLeft) (Some (EARecvJump pc rs mem)) (APFRecvL pc rs mem)
+| APFRecvJumpR pc rs mem:
   pc ∉ ins1 →
   pc ∈ ins2 →
   rs !! "PC" = Some pc →
-  asm_prod_filter ins1 ins2 APFNone (SPENone SPRight) (Some (EARecvJump pc rs)) (APFRecvR pc rs)
+  asm_prod_filter ins1 ins2 APFNone (SPENone SPRight) (Some (EARecvJump pc rs mem)) (APFRecvR pc rs mem)
 .
 
 Definition asm_prod (ins1 ins2 : gset Z) (m1 m2 : module asm_event) : module asm_event :=
@@ -186,14 +250,14 @@ Lemma asm_prod_trefines m1 m1' m2 m2' σ1 σ1' σ2 σ2' ins1 ins2 `{!VisNoAll m1
 Proof. move => ??. apply mod_map_trefines. by apply mod_seq_product_trefines. Qed.
 
 Definition asm_link_prod_inv (ins1 ins2 : gmap Z asm_instr) (σ1 : asm_module.(m_state)) (σ2 : ((seq_product_state * asm_state * asm_state) * asm_prod_filter_state)) : Prop :=
-  let 'AsmState i1 rs1 ins1' := σ1 in
-  let '((σsp, AsmState il rsl insl, AsmState ir rsr insr), σf) := σ2 in
+  let 'AsmState i1 rs1 mem1 ins1' := σ1 in
+  let '((σsp, AsmState il rsl meml insl, AsmState ir rsr memr insr), σf) := σ2 in
   ins1' = ins1 ∪ ins2 ∧
   insl = ins1 ∧
   insr = ins2 ∧
   match σf with
-  | APFLeft => σsp = SPLeft ∧ is_Some i1 ∧ il = i1 ∧ rsl = rs1 ∧ ir = None
-  | APFRight => σsp = SPRight ∧ is_Some i1 ∧ ir = i1 ∧ rsr = rs1 ∧ il = None
+  | APFLeft => σsp = SPLeft ∧ is_Some i1 ∧ il = i1 ∧ rsl = rs1 ∧ meml = mem1 ∧ ir = None
+  | APFRight => σsp = SPRight ∧ is_Some i1 ∧ ir = i1 ∧ rsr = rs1 ∧ memr = mem1 ∧ il = None
   | APFNone => σsp = SPNone ∧ i1 = None ∧ ir = None ∧ il = None
   | _ => False
   end.
@@ -208,54 +272,51 @@ Proof.
   apply tsim_implies_trefines => /= n.
   unshelve apply: tsim_remember. { exact: (λ _, asm_link_prod_inv ins1 ins2). }
   { naive_solver. } { done. }
-  move => /= {}n _ Hloop [i1 rs1 ins1'] [[[? [il rsl insl]] [ir rsr insr] σf]] [? [? [? Hinv]]].
+  move => /= {}n _ Hloop [i1 rs1 mem1 ins1'] [[[? [il rsl meml insl]] [ir rsr memr insr] σf]] [? [? [? Hinv]]].
   case_match; destruct_all?; simplify_eq.
-  - revert select (is_Some i1) => -[[|[??]?] ->].
+  - revert select (is_Some i1) => -[[|[??|???|???]?] ->].
     + tstep_i => pc ?. case_match as Hunion. 1: move: Hunion => /lookup_union_Some_raw[Hl|[? Hl]].
       * tstep_s. eexists _. split; [done|]. simplify_option_eq.
         eexists _. split; [done|]. eexists _, _. split; [done|] => /=.
         apply: Hloop. naive_solver.
-      * tstep_s. eexists _. split; [done|]. simplify_option_eq.
-        eexists _. split; [done|]. eexists _, _. split; [econs|].
+      * tstep_s. split!; [done|]. simplify_option_eq. split!; [econs|].
         { by apply not_elem_of_dom. } { by apply elem_of_dom. } simpl.
-        tstep_s. eexists _, _, _. split; [done|]. split; [done|]. eexists _. split; [done|].
-        eexists _, _. split; [econs|]. simpl.
+        tstep_s. split!; [done|done|econs|]. simpl.
         apply: Hloop. naive_solver.
-      * move: Hunion => /lookup_union_None[??]. tstep_s. eexists _. split; [done|]. simplify_option_eq.
-        eexists _. split; [done|]. eexists _, _. split; [by apply APFJumpExtL; apply not_elem_of_dom|] => /=.
-        split; [done|]. apply: Hloop. naive_solver.
-    + tstep_both. tstep_s. eexists _. split; [done|]. eexists _, _. split; [done|] => /= ?.
-      tend. split; [done|]. apply: Hloop. naive_solver.
-  - revert select (is_Some i1) => -[[|[??]?] ->].
+      * move: Hunion => /lookup_union_None[??]. tstep_s.
+        split!; [done|]. simplify_option_eq.
+        split!; [by apply APFJumpExtL; apply not_elem_of_dom|] => /=. split!.
+        apply: Hloop. naive_solver.
+    + tstep_both. tstep_s. split! => /= ?. tend. split!. apply: Hloop. naive_solver.
+    + tstep_both. tstep_s. split! => /= *. tend. split!; [done..|]. apply: Hloop. naive_solver.
+    + tstep_both. tstep_s. split! => /= *. tend. split!; [done..|]. apply: Hloop. naive_solver.
+  - revert select (is_Some i1) => -[[|[??|???|???]?] ->].
     + tstep_i => pc ?. case_match as Hunion. 1: move: Hunion => /lookup_union_Some_raw[Hl|[? Hl]].
       * have ?: ins2 !! pc = None by apply: map_disjoint_Some_l.
-        tstep_s. eexists _. split; [done|]. simplify_option_eq.
-        eexists _. split; [done|]. eexists _, _. split; [econs|] => /=.
-        { by apply elem_of_dom. } { by apply not_elem_of_dom. }
-        tstep_s. eexists _, _, _. split; [done|]. split; [done|]. eexists _. split; [done|].
-        eexists _, _. split; [econs|]. simpl.
+        tstep_s. split!; [done|]. simplify_option_eq. split!; [econs|].
+        { by apply elem_of_dom. } { by apply not_elem_of_dom. } simpl.
+        tstep_s. split!; [done|done|econs|]. simpl.
         apply: Hloop. naive_solver.
-      * tstep_s. eexists _. split; [done|]. simplify_option_eq.
-        eexists _. split; [done|]. eexists _, _. split; [done|] => /=.
+      * tstep_s. split!; [done|]. simplify_option_eq. split! => /=.
         apply: Hloop. naive_solver.
-      * move: Hunion => /lookup_union_None[??]. tstep_s. eexists _. split; [done|]. simplify_option_eq.
-        eexists _. split; [done|]. eexists _, _. split; [by apply APFJumpExtR; apply not_elem_of_dom|] => /=.
-        split; [done|]. apply: Hloop. naive_solver.
-    + tstep_both. tstep_s. eexists _. split; [done|]. eexists _, _. split; [done|] => /= ?.
-      tend. split; [done|]. apply: Hloop. naive_solver.
-  - tstep_i => pc??? /lookup_union_Some_raw[?|[??]].
+      * move: Hunion => /lookup_union_None[??]. tstep_s.
+        split!; [done|]. simplify_option_eq.
+        split!; [by apply APFJumpExtR; apply not_elem_of_dom|] => /=. split!.
+        apply: Hloop. naive_solver.
+    + tstep_both. tstep_s. split! => /= ?. tend. split!. apply: Hloop. naive_solver.
+    + tstep_both. tstep_s. split! => /= *. tend. split!; [done..|]. apply: Hloop. naive_solver.
+    + tstep_both. tstep_s. split! => /= *. tend. split!; [done..|]. apply: Hloop. naive_solver.
+  - tstep_i => pc???? /lookup_union_Some_raw[?|[??]].
     + have ?: ins2 !! pc = None by apply: map_disjoint_Some_l.
       tstep_s. eexists SPLeft, _, _. split; [econs|] => /=.
       { by apply elem_of_dom. } { by apply not_elem_of_dom. } { done. }
       split; [done|].
-      tstep_s. eexists _, _, _. split; [done|]. split; [done|]. eexists _. split; [done|].
-      eexists _, _. split; [econs|] => /=.
+      tstep_s. split!; [done|done|econs|] => /=.
       apply: Hloop. naive_solver.
     + tstep_s. eexists SPRight, _, _. split; [econs|] => /=.
       { by apply not_elem_of_dom. } { by apply elem_of_dom. } { done. }
       split; [done|].
-      tstep_s. eexists _, _, _. split; [done|]. split; [done|]. eexists _. split; [done|].
-      eexists _, _. split; [econs|] => /=.
+      tstep_s. split!; [done|done|econs|] => /=.
       apply: Hloop. naive_solver.
 Qed.
 
@@ -268,9 +329,9 @@ Proof.
   apply tsim_implies_trefines => /= n.
   unshelve apply: tsim_remember. { exact: (λ _, flip (asm_link_prod_inv ins1 ins2)). }
   { naive_solver. } { done. }
-  move => /= {}n _ Hloop [[[σsp [il rsl insl]] [ir rsr insr]] σf] [i1 rs1 ins1'] [? [? [? Hinv]]].
+  move => /= {}n _ Hloop [[[σsp [il rsl meml insl]] [ir rsr memr insr]] σf] [i1 rs1 mem1 ins1'] [? [? [? Hinv]]].
   case_match; destruct_all?; simplify_eq.
-  - revert select (is_Some i1) => -[[|[??]?] ->].
+  - revert select (is_Some i1) => -[[|[??|???|???]?] ->].
     + tstep_i => pc ?. case_match => *; destruct_all?; simplify_eq.
       * tstep_s. eexists _. split; [done|]. erewrite lookup_union_Some_l by done.
         apply: Hloop. naive_solver.
@@ -284,7 +345,13 @@ Proof.
     + tstep_both => *. destruct_all!. simplify_eq.
       tstep_s => ?. tend. split; [done|].
       apply: Hloop. naive_solver.
-  - revert select (is_Some i1) => -[[|[??]?] ->].
+    + tstep_both => *. destruct_all!. simplify_eq.
+      tstep_s => *. tend. split!; [done..|].
+      apply: Hloop. naive_solver.
+    + tstep_both => *. destruct_all!. simplify_eq.
+      tstep_s => *. tend. split!; [done..|].
+      apply: Hloop. naive_solver.
+  - revert select (is_Some i1) => -[[|[??|???|???]?] ->].
     + tstep_i => pc ?. case_match => *; destruct_all?; simplify_eq.
       * tstep_s. eexists _. split; [done|]. erewrite lookup_union_Some_r by done.
         apply: Hloop. naive_solver.
@@ -298,9 +365,15 @@ Proof.
     + tstep_both => *. destruct_all!. simplify_eq.
       tstep_s => ?. tend. split; [done|].
       apply: Hloop. naive_solver.
+    + tstep_both => *. destruct_all!. simplify_eq.
+      tstep_s => *. tend. split!; [done..|].
+      apply: Hloop. naive_solver.
+    + tstep_both => *. destruct_all!. simplify_eq.
+      tstep_s => *. tend. split!; [done..|].
+      apply: Hloop. naive_solver.
   - tstep_i => *. invert_all asm_prod_filter; tstep_s.
     all: revert select (pc ∈ dom _ _) => /elem_of_dom[??].
-    all: eexists _, _, _; split_and!; [done|by simplify_map_eq|done|].
+    all: eexists _,_, _, _; split_and!; [done|by simplify_map_eq|done|].
     all: tstep_i => *; invert_all asm_prod_filter.
     all: apply: Hloop; try naive_solver.
 Qed.
@@ -331,73 +404,78 @@ Local Ltac go_i :=
 (* TODO: Get rid of Some in recursive call (maybe by passing an itree to t instead of the +'? ) *)
 (* TODO: prove merging of two asm loops (should just be all choice between the two implementations ) *)
 Definition asm_loop (ins : list Z)
-   (t : Z → gmap string Z → itree (callE
-     (option (Z * gmap string Z)) (Z * gmap string Z) +' moduleE asm_event unit) (Z * gmap string Z))
+   (t : Z → gmap string Z → gmap Z Z → itree (callE
+     (option (Z * gmap string Z * gmap Z Z)) (Z * gmap string Z * gmap Z Z) +' moduleE asm_event unit) (Z * gmap string Z * gmap Z Z))
   : itree (moduleE asm_event unit) unit :=
   rec (λ a,
-    '(pc, rs) ← (
-       if a is Some (npc, nrs) then
+    '(pc, rs, mem) ← (
+       if a is Some (npc, nrs, nmem) then
          if bool_decide (npc ∈ ins) then
-           Ret (npc, nrs)
+           Ret (npc, nrs, nmem)
          else
-           translate (inr_) (TVis (EAJump npc nrs));;;;
+           translate (inr_) (TVis (EAJump npc nrs nmem));;;;
            pc ← translate (inr_) (TExist Z);;;
            rs ← translate (inr_) (TExist _);;;
-           translate (inr_) (TVis (EARecvJump pc rs));;;;
-           Ret (pc, rs)
+           mem ← translate (inr_) (TExist _);;;
+           translate (inr_) (TVis (EARecvJump pc rs mem));;;;
+           Ret (pc, rs, mem)
         else
           pc ← translate (inr_) (TExist Z);;;
           rs ← translate (inr_) (TExist _);;;
-          translate (inr_) (TVis (EARecvJump pc rs));;;;
-          Ret (pc, rs)
+          mem ← translate (inr_) (TExist _);;;
+          translate (inr_) (TVis (EARecvJump pc rs mem));;;;
+          Ret (pc, rs, mem)
      );;;
     translate (inr_) (TAssert (pc ∈ ins));;;;
     (* The env can choose if this call should be treated as a call or a return. *)
     b ← translate (inr_) (TAll bool);;;
-    if b then Ret (pc, rs) else
-      r ← t pc rs;;;
+    if b then Ret (pc, rs, mem) else
+      r ← t pc rs mem;;;
       call (Some r)
     ) None;;;; TUb.
 
-Lemma tsim_asm_loop n b rs ins t insaddrs:
+Lemma tsim_asm_loop n b rs mem ins t insaddrs:
   (∀ z, z ∈ insaddrs ↔ is_Some (ins !! z)) →
-  (∀ n rc pc' rs' i k,
+  (∀ n rc pc' rs' mem' i k,
       rs' !! "PC" = Some pc' →
       ins !! pc' = Some i →
-      (∀ pc'' rs1'' rs2'' h',
+      (∀ pc'' rs1'' rs2'' mem1'' mem2'' h',
          rs1'' = rs2'' →
+         mem1'' = mem2'' →
          rs1'' !! "PC" = Some pc'' →
-          (∀ pc''' rs''' i,
+          (∀ pc''' rs''' mem''' i,
               rs''' !! "PC" = Some pc''' → ins !! pc''' = Some i →
-              AsmState (Some i) rs''' ins ⪯{asm_module, mod_itree asm_event (), n, b} (h' (pc''', rs'''), ())) →
-          (AsmState (Some []) rs1'' ins)
+              AsmState (Some i) rs''' mem''' ins ⪯{asm_module, mod_itree asm_event (), n, b} (h' (pc''', rs''', mem'''), ())) →
+          (AsmState (Some []) rs1'' mem1'' ins)
             ⪯{asm_module, mod_itree asm_event (), n, true}
-          (y ← rec rc (Some (pc'', rs2''));;; h' y, ())) →
-      (∀ pc rs1 rs2,
+          (y ← rec rc (Some (pc'', rs2'', mem2''));;; h' y, ())) →
+      (∀ pc rs1 rs2 mem1 mem2,
           rs1 = rs2 →
+          mem1 = mem2 →
           rs1 !! "PC" = Some pc →
-          tsim n true asm_module (mod_itree asm_event ()) (AsmState (Some []) rs1 ins) tnil (k (pc, rs2), ())) →
-    AsmState (Some i) rs' ins ⪯{asm_module, mod_itree asm_event (), n, true}
-       (r ← interp (recursive rc) (t pc' rs');;; k r, ())) →
+          tsim n true asm_module (mod_itree asm_event ()) (AsmState (Some []) rs1 mem1 ins) tnil (k (pc, rs2, mem2), ())) →
+    AsmState (Some i) rs' mem' ins ⪯{asm_module, mod_itree asm_event (), n, true}
+       (r ← interp (recursive rc) (t pc' rs' mem');;; k r, ())) →
   (** Then we can prove an asm_loop *)
-  AsmState None rs ins ⪯{asm_module, mod_itree asm_event (), n, b} (asm_loop insaddrs t, ()).
+  AsmState None rs mem ins ⪯{asm_module, mod_itree asm_event (), n, b} (asm_loop insaddrs t, ()).
 Proof.
   rewrite /asm_loop => Hins Hl. set rc := (X in (rec X)).
   apply (tsim_remember_rec (mi:=asm_module)
    (λ a σi s,
-     if a is Some (pc, rs) then
-       σi = AsmState (Some []) rs ins ∧ rs !! "PC" = Some pc
+     if a is Some (pc, rs, mem) then
+       σi = AsmState (Some []) rs mem ins ∧ rs !! "PC" = Some pc
      else
-       ∃ rs, σi = AsmState None rs ins
+       ∃ rs mem, σi = AsmState None rs mem ins
    )
-   (λ σi '(pc, rs) s', ∃ i, σi = AsmState (Some i) rs ins ∧ rs !! "PC" = Some pc ∧ ins !! pc = Some i)).
+   (λ σi '(pc, rs, mem) s', ∃ i, σi = AsmState (Some i) rs mem ins ∧ rs !! "PC" = Some pc ∧ ins !! pc = Some i)).
   { naive_solver. }
   { move => ????. go_s. done. }
   move => {}n _ Hloop σi [] CONT a Ha HCONT.
-  destruct a as [[pc' rs']|]. 2: {
-    move: Ha => [{}rs ?]. subst.
-    tstep_i => pc i {}rs HPC Hi.
+  destruct a as [[[pc' rs'] mem']|]. 2: {
+    move: Ha => [{}rs [{}mem ?]]. subst.
+    tstep_i => pc i {}rs {}mem HPC Hi.
     rewrite {1}rec_as_interp {2}/rc.
+    go_s. eexists _. go.
     go_s. eexists _. go.
     go_s. eexists _. go.
     go_s. split; [done|]. go.
@@ -406,11 +484,11 @@ Proof.
     { go_s. apply: tsim_mono_b. revert select (eqit eq _ _ _ _) => ->. apply HCONT. naive_solver. }
     revert select (eqit eq _ _ _ _) => ->. rewrite interp_bind bind_bind.
     apply: Hl; [done..| |].
-    - move => ???????. subst. apply Hloop; [done|].
-      move => ? [rs' pc'] []. naive_solver.
-    - move => ?????. rewrite interp_recursive_call.
+    - move => ??????????. subst. apply Hloop; [done|].
+      move => ? [[rs' pc'] mem'] []. naive_solver.
+    - move => ????????. rewrite interp_recursive_call.
       apply Hloop. { naive_solver. }
-      move => ? [??] [] [?[??]]. apply: HCONT. naive_solver.
+      move => ? [[??]?] [] [?[??]]. apply: HCONT. naive_solver.
   }
   destruct Ha. simplify_eq.
   tstep_i => pc HPC. simplify_eq.
@@ -421,14 +499,15 @@ Proof.
     { go_s. apply: tsim_mono_b. revert select (eqit eq _ _ _ _) => ->. apply HCONT. naive_solver. }
     revert select (eqit eq _ _ _ _) => ->. rewrite interp_bind bind_bind.
     apply: Hl; [done..| |].
-    + move => ???????. subst. apply Hloop; [done|].
-      move => ? [? ?] []. naive_solver.
-    + move => ?????. rewrite interp_recursive_call.
+    + move => ??????????. subst. apply Hloop; [done|].
+      move => ? [[??] ?] []. naive_solver.
+    + move => ????????. rewrite interp_recursive_call.
       apply Hloop. { naive_solver. }
-      move => ? [??] [] [?[??]]. apply: HCONT. naive_solver.
+      move => ? [[??]?] [] [?[??]]. apply: HCONT. naive_solver.
   - rewrite {1}rec_as_interp {2}/rc. rewrite bool_decide_false. { move => /Hins[??]. naive_solver. }
     go_s. split; [done|]. go.
-    tstep_i => pc i {}rs HPC Hi.
+    tstep_i => pc i {}rs {}mem HPC Hi.
+    go_s. eexists _. go.
     go_s. eexists _. go.
     go_s. eexists _. go.
     go_s. split; [done|]. go.
@@ -437,11 +516,11 @@ Proof.
     { go_s. apply: tsim_mono_b. revert select (eqit eq _ _ _ _) => ->. apply HCONT. naive_solver. }
     revert select (eqit eq _ _ _ _) => ->. rewrite interp_bind bind_bind.
     apply: Hl; [done..| |].
-    + move => ???????. subst. apply Hloop; [done|].
-      move => ? [? ?] []. naive_solver.
-    + move => ?????. rewrite interp_recursive_call.
+    + move => ??????????. subst. apply Hloop; [done|].
+      move => ? [[??] ?] []. naive_solver.
+    + move => ????????. rewrite interp_recursive_call.
       apply Hloop. { naive_solver. }
-      move => ? [??] [] [?[??]]. apply: HCONT. naive_solver.
+      move => ? [[??]?] [] [?[??]]. apply: HCONT. naive_solver.
 Qed.
 
 Module asm_examples.
@@ -458,12 +537,12 @@ Module asm_examples.
       ] ]> $ ∅.
 
   Definition itree_mul : itree (moduleE asm_event unit) unit :=
-    asm_loop [100; 104] (λ pc rs,
+    asm_loop [100; 104] (λ pc rs mem,
        if bool_decide (pc = 100) then
          r1 ← translate (inr_) (TAssumeOpt (rs !! "R1"));;;
          r2 ← translate (inr_) (TAssumeOpt (rs !! "R2"));;;
          r30 ← translate (inr_) (TAssumeOpt (rs !! "R30"));;;
-         Ret (r30, (<["PC":=r30]> $ <["R1":=r1 * r2]> $ rs))
+         Ret (r30, (<["PC":=r30]> $ <["R1":=r1 * r2]> $ rs), mem)
        else if bool_decide (pc = 104) then
          translate (inr_) TUb
        else
@@ -481,7 +560,7 @@ Module asm_examples.
       rewrite !lookup_insert_is_Some' lookup_empty -not_eq_None_Some.
       naive_solver.
     }
-    move => {}n rc pc rs i CONT HPC Hi Hloop HCONT.
+    move => {}n rc pc rs mem i CONT HPC Hi Hloop HCONT.
     move: Hi. rewrite !lookup_insert_Some !lookup_empty => Hi. destruct_all!; simplify_eq.
     all: repeat (rewrite bool_decide_false; [done|]); rewrite bool_decide_true //.
     all: try by go_s.
@@ -526,7 +605,7 @@ Module asm_examples.
       ] ]> $ ∅.
 
   Definition itree_mul_client : itree (moduleE asm_event unit) unit :=
-    asm_loop [200; 204; 208; 212; 216] (λ pc rs,
+    asm_loop [200; 204; 208; 212; 216] (λ pc rs mem,
        if bool_decide (pc = 200) then
          translate (inr_) (TAssume (is_Some (rs !! "R1")));;;;
          translate (inr_) (TAssume (is_Some (rs !! "R2")));;;;
@@ -534,14 +613,14 @@ Module asm_examples.
          r30 ← translate (inr_) (TAssumeOpt (rs !! "R30"));;;
          r29' ← translate (inr_) (TExist Z);;;
          (* translate (inr_) (TVis (EAJump 100 (<["PC":=100]> $ <["R30":= 212]> $ <["R29":= r29']> $ <["R2":= 2]> $ <["R1":= 2]> $ rs)));;;; *)
-         '(pc', rs') ← call (Some (100, (<["PC":=100]> $ <["R30":= 212]> $ <["R29":= r29']> $ <["R2":= 2]> $ <["R1":= 2]> $ rs)));;;
+         '(pc', rs', mem') ← call (Some (100, (<["PC":=100]> $ <["R30":= 212]> $ <["R29":= r29']> $ <["R2":= 2]> $ <["R1":= 2]> $ rs), mem));;;
          translate (inr_) (TAssume (pc' = 212));;;;
          translate (inr_) (TAssume (is_Some (rs' !! "R30")));;;;
          translate (inr_) (TAssume (rs' !! "R29" = Some r29'));;;;
          translate (inr_) (TAssume (r30 ≠ 200 ∧ r30 ≠ 204 ∧ r30 ≠ 208 ∧ r30 ≠ 212 ∧ r30 ≠ 216));;;;
          r30' ← translate (inr_) (TExist Z);;;
          (* translate (inr_) (TVis (EAJump r30 (<["PC":= r30]> $ <["R30":= r30']> rs')));;;; *)
-         Ret (r30, (<["PC":= r30]> $ <["R30":= r30']> rs'))
+         Ret (r30, (<["PC":= r30]> $ <["R30":= r30']> rs'), mem')
        else if bool_decide (pc = 204) then translate (inr_) TUb
        else if bool_decide (pc = 208) then translate (inr_) TUb
        else if bool_decide (pc = 212) then translate (inr_) TUb
@@ -560,7 +639,7 @@ Module asm_examples.
       rewrite !lookup_insert_is_Some' lookup_empty -not_eq_None_Some.
       naive_solver.
     }
-    move=> {}n rc pc rs i CONT HPC Hi Hloop HCONT.
+    move=> {}n rc pc rs mem i CONT HPC Hi Hloop HCONT.
     move: Hi. rewrite !lookup_insert_Some !lookup_empty => Hi. destruct_all!; simplify_eq.
     all: repeat (rewrite bool_decide_false; [done|]); rewrite bool_decide_true //.
     all: try by go_s.
@@ -583,8 +662,8 @@ Module asm_examples.
     go_s. eexists r30; go.
     go_s.
     revert select (eqit eq _ _ _ _) => ->.
-    apply Hloop. { by sort_map_insert. } { by simplify_map_eq. }
-    move => pc' rs'' i HPC' Hi'.
+    apply Hloop. { by sort_map_insert. } { done. } { by simplify_map_eq. }
+    move => pc' rs'' mem'' i HPC' Hi'.
     go_s => ?; go; subst. unfold asm_mul_client in Hi'. simplify_map_eq.
     go_s => -[r30'' HR30'']; go.
     go_s => ?; go.
@@ -595,6 +674,6 @@ Module asm_examples.
     tstep_i; simplify_map_eq'. split!.
     go_s. eexists _; go.
     go_s. revert select (eqit eq _ _ _ _) => ->.
-    apply HCONT; [done|]. by simplify_map_eq.
+    apply HCONT; [done..|]. by simplify_map_eq.
   Qed.
 End asm_examples.
