theories/imp_to_asm_examples.v
@@ -43,8 +43,9 @@ Definition asm_add_client : gmap Z asm_instr :=
         WriteReg "PC" (λ rs, rs !!! "PC" + 4)
     ] ]> $
   <[ 208 := [
-        (* mov R29, R30 *)
-        WriteReg "R29" (λ rs, rs !!! "R30");
+        (* push R30 *)
+        WriteReg "SP" (λ rs, rs !!! "SP" - 1);
+        WriteMem "R30" "SP" id;
         WriteReg "PC" (λ rs, rs !!! "PC" + 4)
     ] ]> $
   <[ 212 := [
@@ -53,8 +54,14 @@ Definition asm_add_client : gmap Z asm_instr :=
         WriteReg "PC" (λ rs, 100)
     ] ]> $
   <[ 216 := [
+        (* pop R30 *)
+        ReadMem "R30" "SP" id;
+        WriteReg "SP" (λ rs, rs !!! "SP" + 1);
+        WriteReg "PC" (λ rs, rs !!! "PC" + 4)
+    ] ]> $
+  <[ 220 := [
         (* ret *)
-        WriteReg "PC" (λ rs, rs !!! "R29")
+        WriteReg "PC" (λ rs, rs !!! "R30")
     ] ]> $ ∅.
 
 Definition imp_add_client : fndef := {|
@@ -73,10 +80,10 @@ Local Ltac go_s := tstep_s; go.
 
 Lemma asm_add_refines_imp_add :
   trefines (MS asm_module (initial_asm_state asm_add))
-           (MS (imp_to_asm imp_module) (initial_imp_to_asm_state imp_module (initial_imp_state imp_add_prog) {[ 100; 104 ]} {[ "add" ]} (<["add" := 100]> ∅))).
+           (MS (imp_to_asm imp_module) (initial_imp_to_asm_state imp_module (initial_imp_state imp_add_prog) (dom _ asm_add) (dom _ imp_add_prog) (<["add" := 100]> ∅))).
 Proof.
   apply imp_to_asm_proof; [set_solver..|].
-  move => n i rs K f fn vs cs t pc ret Hpc Hi Hf Hf2i Hargs Hvs Hcall Hret.
+  move => n i rs mem K f fn vs cs t pc ret Hpc Hi Hf Hf2i Hargs Hvs Hcall Hret.
   unfold imp_add_prog in Hf. unfold asm_add in Hi.
   move: Hf2i. rewrite !lookup_insert_Some => ?; destruct_all?; simplify_map_eq/=.
   destruct vs as [|v1 [|v2 []]] => //=.
@@ -95,11 +102,11 @@ Qed.
 Lemma asm_add_client_refines_imp_add_client :
   trefines (MS asm_module (initial_asm_state asm_add_client))
            (MS (imp_to_asm imp_module) (initial_imp_to_asm_state imp_module
-          (initial_imp_state imp_add_client_prog) {[ 200; 204; 208; 212; 216 ]} {[ "add_client" ]}
-          (<["add_client" := 200]> $ <["add" := 100]> ∅))).
+          (initial_imp_state imp_add_client_prog) (dom _ asm_add_client)
+          (dom _ imp_add_client_prog) (<["add_client" := 200]> $ <["add" := 100]> ∅))).
 Proof.
   apply imp_to_asm_proof; [set_solver..|].
-  move => n i rs K f fn vs cs t pc ret Hpc Hi Hf Hf2i Hargs Hvs Hcall Hret.
+  move => n i rs mem K f fn vs cs t pc ret Hpc Hi Hf Hf2i Hargs Hvs Hcall Hret.
   unfold imp_add_client_prog in Hf. unfold asm_add_client in Hi.
   move: Hf2i. rewrite !lookup_insert_Some => ?; destruct_all?; simplify_map_eq/=.
   destruct vs as [|] => //=.
@@ -111,7 +118,8 @@ Proof.
   tstep_i; simplify_map_eq'. split; [done|].
   tstep_i => ??. simplify_map_eq'.
   tstep_i; simplify_map_eq'. split; [done|].
-  tstep_i; simplify_map_eq'. split; [done|].
+  tstep_i; simplify_map_eq'. split!; [done..|].
+  tstep_i; simplify_map_eq'. split!; [done..|].
   tstep_i => ??. simplify_map_eq'.
   tstep_i; simplify_map_eq'. split; [done|].
   tstep_i; simplify_map_eq'. split; [done|].
@@ -120,13 +128,18 @@ Proof.
   apply: Hcall. { repeat econs. } { by simplify_map_eq. } { set_solver. } { set_solver. } { by simplify_map_eq. }
   { unfold imp_to_asm_args. unfold tmp_registers, saved_registers.
     split!; decompose_Forall; simplify_map_eq => //. } { by simplify_map_eq. } { done. }
-  move => rs'' v ? Hpc'' Hv ?.
+  move => rs'' mem'' v ? Hpc'' Hv ?.
   move: Hv => -[?[/= ? Hregs]]. unfold tmp_registers, saved_registers in *. decompose_Forall_hyps.
   simplify_map_eq'.
+  tstep_i; simplify_map_eq'. split!; [done..|].
+  tstep_i; simplify_map_eq'. split!; [done..|].
+  tstep_i; simplify_map_eq'. split!; [done..|].
+  tstep_i => ??. simplify_map_eq'.
   tstep_i; simplify_map_eq'. split; [done|].
-  apply: Hret; [by simplify_map_eq'| |done].
+  apply: Hret; [| |done]. { simplify_map_eq'. admit. }
   unfold imp_to_asm_ret. unfold tmp_registers, saved_registers.
   split!; decompose_Forall; simplify_map_eq => //.
+  f_equal. lia.
   (* TODO: without a stack one cannot save the original frame pointer anywhere *)
 Admitted.
 
@@ -139,7 +152,7 @@ Definition full_imp_add : gmap string fndef :=
 Lemma full_add_stack :
   trefines (MS asm_module (initial_asm_state full_asm_add))
            (MS (imp_to_asm imp_module) (initial_imp_to_asm_state imp_module
-              (initial_imp_state full_imp_add) {[ 100; 104; 200; 204; 208; 212; 216 ]} {[ "add"; "add_client" ]}
+              (initial_imp_state full_imp_add) {[ 100; 104; 200; 204; 208; 212; 216; 220 ]} {[ "add"; "add_client" ]}
               (<["add_client" := 200]> $ <["add" := 100]> ∅))).
 Proof.
   etrans. { apply asm_link_refines_prod. unfold asm_add, asm_add_client. eauto with map_disjoint. }
@@ -149,8 +162,6 @@ Proof.
     - apply asm_add_client_refines_imp_add_client.
   }
   etrans. {
-    have ->: (dom (gset Z) asm_add) = {[100; 104]} by set_solver.
-    have ->: (dom (gset Z) asm_add_client) = {[200; 204; 208; 212; 216]} by set_solver.
     apply imp_to_asm_combine.
     - apply _.
     - apply _.
@@ -164,12 +175,10 @@ Proof.
   }
   etrans. {
     apply imp_to_asm_trefines. { apply _. }
-    have <-: (dom (gset _) imp_add_prog) = {["add"]} by set_solver.
-    have <-: (dom (gset _) imp_add_client_prog) = {["add_client"]} by set_solver.
     apply imp_prod_refines_link.
     unfold imp_add_prog, imp_add_client_prog. eauto with map_disjoint.
   }
-  f_equiv. f_equal. { set_solver. }
+  f_equiv. f_equal. { set_solver. } { set_solver. }
   rewrite -insert_union_r. set_solver.
   f_equal.
   apply idemp.
